src/QUIC.Secret.Buffer.fsti
@@ -60,6 +60,229 @@ val with_buffer_hide
     post res (B.as_seq h' (B.gsub b 0ul from)) (B.as_seq h' (B.gsub b from (to `U32.sub` from))) (B.as_seq h' (B.gsub b to (B.len b `U32.sub` to))) h'
   ))
 
+(* NOTE: this CANNOT be derived from with_buffer_hide, because the footprint of a zero-length buffer is not B.loc_none *)
+
+inline_for_extraction
+noextract
+val with_buffer_hide_weak_modifies
+  (#t: Type)
+  (b: B.buffer U8.t)
+  (from: U32.t)
+  (to: U32.t { U32.v from <= U32.v to /\ U32.v to <= B.length b })
+  (h0: HS.mem)
+  (lin: Ghost.erased B.loc { B.loc_disjoint (Ghost.reveal lin) (B.loc_buffer b) })
+  (lout: Ghost.erased B.loc { B.loc_disjoint (Ghost.reveal lout) (B.loc_buffer b) })
+  (modifies_left modifies_secret modifies_right: Ghost.erased bool)
+  (post: (res: t) ->  (contl: Seq.lseq U8.t (U32.v from)) ->  (cont: Seq.lseq U8.t (U32.v to - U32.v from)) ->  (contr: Seq.lseq U8.t (B.length b - U32.v to)) -> (h: HS.mem) -> GTot Type0)
+  (f: (
+    (l: Ghost.erased B.loc) ->
+    (bl: B.buffer U8.t { B.length bl == (U32.v from) }) ->
+    (bs: B.buffer Secret.uint8 { B.length bs == (U32.v to - U32.v from) }) ->
+    (br: B.buffer U8.t { B.length br == (B.length b - U32.v to) }) ->
+    HST.Stack t
+    (requires (fun h ->
+      B.modifies l h0 h /\
+      B.loc_disjoint (B.loc_buffer bl `B.loc_union` B.loc_buffer bs) (B.loc_buffer br) /\
+      B.loc_disjoint (B.loc_buffer bl) (B.loc_buffer bs) /\
+      B.loc_disjoint (Ghost.reveal lin `B.loc_union` Ghost.reveal lout) (Ghost.reveal l `B.loc_union` B.loc_buffer bl `B.loc_union` B.loc_buffer bs `B.loc_union` B.loc_buffer br) /\
+      B.live h bl /\ B.live h bs /\ B.live h br /\
+      B.as_seq h bl == B.as_seq h0 (B.gsub b 0ul from) /\
+      B.as_seq h bs == Seq.seq_hide #Secret.U8 (B.as_seq h0 (B.gsub b from (to `U32.sub` from))) /\
+      B.as_seq h br == B.as_seq h0 (B.gsub b to (B.len b `U32.sub` to))
+    ))
+    (ensures (fun h res h' ->
+      B.modifies (Ghost.reveal lout `B.loc_union` (if Ghost.reveal modifies_left then B.loc_buffer bl else B.loc_none) `B.loc_union` (if Ghost.reveal modifies_secret then B.loc_buffer bs else B.loc_none) `B.loc_union` (if Ghost.reveal modifies_right then B.loc_buffer br else B.loc_none)) h h' /\
+      post res (B.as_seq h' bl) (Seq.seq_reveal (B.as_seq h' bs)) (B.as_seq h' br) h'
+    ))
+  ))
+: HST.Stack t
+  (requires (fun h ->
+    B.live h b /\
+    h0 == h
+  ))
+  (ensures (fun h res h' ->
+    B.modifies (Ghost.reveal lout `B.loc_union` (if Ghost.reveal modifies_left then B.loc_buffer (B.gsub b 0ul from) else B.loc_none) `B.loc_union` (if Ghost.reveal modifies_secret then B.loc_buffer (B.gsub b from (to `U32.sub` from)) else B.loc_none) `B.loc_union` (if Ghost.reveal modifies_right then B.loc_buffer (B.gsub b to (B.len b `U32.sub` to)) else B.loc_none)) h h' /\
+    post res (B.as_seq h' (B.gsub b 0ul from)) (B.as_seq h' (B.gsub b from (to `U32.sub` from))) (B.as_seq h' (B.gsub b to (B.len b `U32.sub` to))) h'
+  ))
+
+inline_for_extraction
+noextract
+val with_buffer_hide_from
+  (#t: Type)
+  (b: B.buffer U8.t)
+  (from: U32.t { U32.v from <= B.length b })
+  (h0: HS.mem)
+  (lin: Ghost.erased B.loc { B.loc_disjoint (Ghost.reveal lin) (B.loc_buffer b) })
+  (lout: Ghost.erased B.loc { B.loc_disjoint (Ghost.reveal lout) (B.loc_buffer b) })
+  (x1 x2 x3: Ghost.erased U32.t)
+  (x4: Ghost.erased U32.t {
+    U32.v x1 <= U32.v x2 /\ U32.v x2 <= U32.v from /\
+    U32.v x3 <= U32.v x4 /\ U32.v x4 <= B.length b - U32.v from
+  })
+  (post: (res: t) ->  (contl: Seq.lseq U8.t (U32.v from)) ->  (cont: Seq.lseq U8.t (B.length b - U32.v from)) -> (h: HS.mem) -> GTot Type0)
+  (f: (
+    (l: Ghost.erased B.loc) ->
+    (bl: B.buffer U8.t { B.length bl == (U32.v from) }) ->
+    (bs: B.buffer Secret.uint8 { B.length bs == (B.length b - U32.v from) }) ->
+    HST.Stack t
+    (requires (fun h ->
+      B.modifies l h0 h /\
+      B.loc_disjoint (B.loc_buffer bl) (B.loc_buffer bs) /\
+      B.loc_disjoint (Ghost.reveal lin `B.loc_union` Ghost.reveal lout) (Ghost.reveal l `B.loc_union` B.loc_buffer bl `B.loc_union` B.loc_buffer bs) /\
+      B.live h bl /\ B.live h bs /\
+      B.as_seq h bl == B.as_seq h0 (B.gsub b 0ul from) /\
+      B.as_seq h bs == Seq.seq_hide #Secret.U8 (B.as_seq h0 (B.gsub b from (B.len b `U32.sub` from)))
+    ))
+    (ensures (fun h res h' ->
+      B.modifies (Ghost.reveal lout `B.loc_union` (if U32.v x1 = U32.v x2 then B.loc_none else B.loc_buffer (B.gsub bl x1 (x2 `U32.sub` x1))) `B.loc_union` (if U32.v x3 = U32.v x4 then B.loc_none else B.loc_buffer (B.gsub bs x3 (x4 `U32.sub` x3)))) h h' /\
+      post res (B.as_seq h' bl) (Seq.seq_reveal (B.as_seq h' bs)) h'
+    ))
+  ))
+: HST.Stack t
+  (requires (fun h ->
+    B.live h b /\
+    h0 == h
+  ))
+  (ensures (fun h res h' ->
+    B.modifies (Ghost.reveal lout `B.loc_union` (if U32.v x1 = U32.v x2 then B.loc_none else B.loc_buffer (B.gsub b x1 (x2 `U32.sub` x1))) `B.loc_union` (if U32.v x3 = U32.v x4 then B.loc_none else B.loc_buffer (B.gsub b (from `U32.add` x3) (x4 `U32.sub` x3)))) h h' /\
+    post res (B.as_seq h' (B.gsub b 0ul from)) (B.as_seq h' (B.gsub b from (B.len b `U32.sub` from))) h'
+  ))
+
+inline_for_extraction
+noextract
+val with_buffer_hide_from_weak_modifies
+  (#t: Type)
+  (b: B.buffer U8.t)
+  (from: U32.t { U32.v from <= B.length b })
+  (h0: HS.mem)
+  (lin: Ghost.erased B.loc { B.loc_disjoint (Ghost.reveal lin) (B.loc_buffer b) })
+  (lout: Ghost.erased B.loc { B.loc_disjoint (Ghost.reveal lout) (B.loc_buffer b) })
+  (modifies_left modifies_secret: Ghost.erased bool)
+  (post: (res: t) ->  (contl: Seq.lseq U8.t (U32.v from)) ->  (cont: Seq.lseq U8.t (B.length b - U32.v from)) -> (h: HS.mem) -> GTot Type0)
+  (f: (
+    (l: Ghost.erased B.loc) ->
+    (bl: B.buffer U8.t { B.length bl == (U32.v from) }) ->
+    (bs: B.buffer Secret.uint8 { B.length bs == (B.length b - U32.v from) }) ->
+    HST.Stack t
+    (requires (fun h ->
+      B.modifies l h0 h /\
+      B.loc_disjoint (B.loc_buffer bl) (B.loc_buffer bs) /\
+      B.loc_disjoint (Ghost.reveal lin `B.loc_union` Ghost.reveal lout) (Ghost.reveal l `B.loc_union` B.loc_buffer bl `B.loc_union` B.loc_buffer bs) /\
+      B.live h bl /\ B.live h bs /\
+      B.as_seq h bl == B.as_seq h0 (B.gsub b 0ul from) /\
+      B.as_seq h bs == Seq.seq_hide #Secret.U8 (B.as_seq h0 (B.gsub b from (B.len b `U32.sub` from)))
+    ))
+    (ensures (fun h res h' ->
+      B.modifies (Ghost.reveal lout `B.loc_union` (if Ghost.reveal modifies_left then B.loc_buffer bl else B.loc_none) `B.loc_union` (if Ghost.reveal modifies_secret then B.loc_buffer bs else B.loc_none)) h h' /\
+      post res (B.as_seq h' bl) (Seq.seq_reveal (B.as_seq h' bs)) h'
+    ))
+  ))
+: HST.Stack t
+  (requires (fun h ->
+    B.live h b /\
+    h0 == h
+  ))
+  (ensures (fun h res h' ->
+    B.modifies (Ghost.reveal lout `B.loc_union` (if Ghost.reveal modifies_left then B.loc_buffer (B.gsub b 0ul from) else B.loc_none) `B.loc_union` (if Ghost.reveal modifies_secret then B.loc_buffer (B.gsub b from (B.len b `U32.sub` from)) else B.loc_none)) h h' /\
+    post res (B.as_seq h' (B.gsub b 0ul from)) (B.as_seq h' (B.gsub b from (B.len b `U32.sub` from))) h'
+  ))
+
+inline_for_extraction
+noextract
+let with_whole_buffer_hide_weak_modifies
+  (#t: Type)
+  (b: B.buffer U8.t)
+  (h0: HS.mem)
+  (lin: Ghost.erased B.loc { B.loc_disjoint (Ghost.reveal lin) (B.loc_buffer b) })
+  (lout: Ghost.erased B.loc { B.loc_disjoint (Ghost.reveal lout) (B.loc_buffer b) })
+  (modifies_b: Ghost.erased bool)
+  (post: (res: t) -> (cont: Seq.lseq U8.t (B.length b)) -> (h: HS.mem) -> GTot Type0)
+  (f: (
+    (l: Ghost.erased B.loc) ->
+    (bs: B.buffer Secret.uint8 { B.length bs == B.length b }) ->
+    HST.Stack t
+    (requires (fun h ->
+      B.modifies l h0 h /\
+      B.loc_disjoint (Ghost.reveal lin `B.loc_union` Ghost.reveal lout) (Ghost.reveal l `B.loc_union` B.loc_buffer bs) /\
+      B.live h bs /\
+      B.as_seq h bs == Seq.seq_hide #Secret.U8 (B.as_seq h0 b)
+    ))
+    (ensures (fun h res h' ->
+      B.modifies (Ghost.reveal lout `B.loc_union` (if Ghost.reveal modifies_b then B.loc_buffer bs else B.loc_none)) h h' /\
+      post res (Seq.seq_reveal (B.as_seq h' bs)) h'
+    ))
+  ))
+: HST.Stack t
+  (requires (fun h ->
+    B.live h b /\
+    h0 == h
+  ))
+  (ensures (fun h res h' ->
+    B.modifies (Ghost.reveal lout `B.loc_union` (if Ghost.reveal modifies_b then B.loc_buffer b else B.loc_none)) h h' /\
+    post res (B.as_seq h' b) h'
+  ))
+= let sq : squash (B.gsub b 0ul (B.len b) == b) =
+    B.gsub_zero_length b
+  in
+  let h0 = HST.get () in
+  with_buffer_hide_from_weak_modifies
+    b
+    0ul
+    h0
+    lin
+    lout
+    (Ghost.hide false) modifies_b
+    (fun res _ cont h -> post res cont h)
+    (fun l bl bs ->
+      f l bs
+    )
+
+inline_for_extraction
+noextract
+let with_whole_buffer_hide_weak_modifies'
+  (#t: Type)
+  (b: B.buffer U8.t)
+  (h0: HS.mem)
+  (lin: Ghost.erased B.loc { B.loc_disjoint (Ghost.reveal lin) (B.loc_buffer b) })
+  (lout: Ghost.erased B.loc { B.loc_disjoint (Ghost.reveal lout) (B.loc_buffer b) })
+  (modifies_b: Ghost.erased bool)
+  (post: (res: t) -> (cont: Seq.lseq Secret.uint8 (B.length b)) -> (h: HS.mem) -> GTot Type0)
+  (f: (
+    (l: Ghost.erased B.loc) ->
+    (bs: B.buffer Secret.uint8 { B.length bs == B.length b }) ->
+    HST.Stack t
+    (requires (fun h ->
+      B.modifies l h0 h /\
+      B.loc_disjoint (Ghost.reveal lin `B.loc_union` Ghost.reveal lout) (Ghost.reveal l `B.loc_union` B.loc_buffer bs) /\
+      B.live h bs /\
+      B.as_seq h bs == Seq.seq_hide #Secret.U8 (B.as_seq h0 b)
+    ))
+    (ensures (fun h res h' ->
+      B.modifies (Ghost.reveal lout `B.loc_union` (if Ghost.reveal modifies_b then B.loc_buffer bs else B.loc_none)) h h' /\
+      post res (B.as_seq h' bs) h'
+    ))
+  ))
+: HST.Stack t
+  (requires (fun h ->
+    B.live h b /\
+    h0 == h
+  ))
+  (ensures (fun h res h' ->
+    B.modifies (Ghost.reveal lout `B.loc_union` (if Ghost.reveal modifies_b then B.loc_buffer b else B.loc_none)) h h' /\
+    post res (Seq.seq_hide (B.as_seq h' b)) h'
+  ))
+= let h0 = HST.get () in
+  with_whole_buffer_hide_weak_modifies
+    b
+    h0
+    lin
+    lout
+    modifies_b
+    (fun res cont h -> post res (Seq.seq_hide #Secret.U8 cont) h)
+    (fun l bs ->
+      f l bs
+    )
+
 module E = FStar.Endianness
 
 inline_for_extraction noextract
@@ -76,6 +299,24 @@ val load32_le
   HST.Stack Secret.uint32
     (requires (fun h -> B.live h b))
     (ensures  (fun h0 z h1 -> h0 == h1 /\ B.live h1 b /\
+                           E.le_to_n (Seq.seq_reveal (B.as_seq h1 b)) == Secret.v z))
+
+inline_for_extraction noextract
+val store32_be
+  (b:B.buffer Secret.uint8 {B.length b == 4})
+  (z:Secret.uint32)
+: HST.Stack unit
+    (requires (fun h -> B.live h b))
+    (ensures  (fun h0 _ h1 -> B.(modifies (loc_buffer b) h0 h1) /\ B.live h1 b /\
+                           E.be_to_n (Seq.seq_reveal (B.as_seq h1 b)) == Secret.v z))
+
+inline_for_extraction noextract
+val store32_le
+  (b:B.buffer Secret.uint8 {B.length b == 4})
+  (z:Secret.uint32)
+: HST.Stack unit
+    (requires (fun h -> B.live h b))
+    (ensures  (fun h0 _ h1 -> B.(modifies (loc_buffer b) h0 h1) /\ B.live h1 b /\
                            E.le_to_n (Seq.seq_reveal (B.as_seq h1 b)) == Secret.v z))
 
 (* Not secret-related, but very useful for footprints *)
